examples/logic/modal-tableaux/modalBasicsScript.sml
@@ -39,7 +39,7 @@ Datatype:
     Var num | NVar num | Conj nnfform nnfform | Disj nnfform nnfform |
     Box nnfform | Dia nnfform
 End
-val _ = export_rewrites ["form_size_def"]
+val _ = export_rewrites ["nnfform_size_def"]
 
 Definition forces_def[simp]:
   (forces M w (Var n)      ⇔ w ∈ M.frame.world ∧ w ∈ M.valt n) ∧
